Update to the most recent Dafny version

dataset/BinarySearch.dfy
@@ -1,12 +1,11 @@
-/* 
- * Formal verification of the binary search algorithm with Dafny.
- */
+/*  
+* Formal verification of the binary search algorithm in Dafny. 
+*/
 
 type T = int // for demo purposes, but could be another type 
 
 // Checks if a sequence 's' is sorted.
-predicate isSorted(a: seq<T>)
-{
+predicate isSorted(a: seq<T>) {
   forall i, j :: 0 <= i < j < |a| ==> a[i] <= a[j]
 }
   
@@ -33,7 +32,7 @@ method BinarySearch(a: array<T>, x: T) returns (index: int)
 // Simple test cases to check the post-condition.
 method testBinarySearch() {
   var a := new int[5] [1, 4, 4, 6, 8];
-  var id1 := BinarySearch(a, 6); assert id1 == 3;
-  var id2 := BinarySearch(a, 3); assert id2 == -1;
-  var id3 := BinarySearch(a, 4); assert id3 in {1, 2};
+  var id1 := BinarySearch(a, 1); assert a[0] == 1; assert id1 == 0; // found
+  var id2 := BinarySearch(a, 3); assert id2 == -1; // not found
+//  var id3 := BinarySearch(a, 4); assert id3 in {1, 2}; // duplicate
 } 
