dataset/task_id_632.dfy
@@ -1,15 +1,14 @@
 // Move all zeroes to the end of the array, preserving the order of non-zero elements.
 method MoveZeroesToEnd(a: array<int>)
     modifies a
-    ensures a[..] == fill(filter(old(a[..]), x => x !=0 ), 0, a.Length)
+    ensures a[..] == fill(filter(old(a[..]), x => x != 0 ), 0, a.Length)
 {
     var nz := 0; // number of non-zero elems to the left of index i
     for i := 0 to a.Length // iterate over the array and swap non-zero elements to the left
         invariant 0 <= nz <= i
         invariant a[..nz] == filter(old(a[..i]), x => x != 0) // first nz elements are non-zero, by the same order
-        invariant forall k :: nz <= k < i ==> a[k] == 0 // then zero up to index i (exclusive)
-        invariant a[i..] == old(a[i..])  // then old values up to the end
-        
+        invariant a[nz..i] == fill([], 0, i - nz) // then zero up to index i (exclusive)
+        invariant a[i..] == old(a[i..])  // then old values up to the end       
     {
         if a[i] != 0 {
             if nz < i {
@@ -24,10 +23,11 @@ method MoveZeroesToEnd(a: array<int>)
 
 // Sequence utilities
 
-// Filters a sequence using a predicate.
-// Returns a new sequence with the elements of s that satisfy the predicate p.
-function filter<T>(s: seq<T>, p: T -> bool): (r : seq<T>)
+// Filters a sequence 's' using a predicate 'p'.
+// Returns a new sequence with the elements of 's' that satisfy the predicate 'p'.
+ghost function filter<T>(s: seq<T>, p: T -> bool): (r : seq<T>)
     ensures |r| <= |s| // useful sometimes    
+    ensures forall i :: 0 <= i < |r| ==> p(r[i])
 {
     if |s| == 0 then s
     else if p(last(s)) then filter(butlast(s), p) + [last(s)]
@@ -35,36 +35,29 @@ function filter<T>(s: seq<T>, p: T -> bool): (r : seq<T>)
 }
 
 // Appens a value (x) to a sequence (s), to fullfil a given length (len).
-// Returns a new sequence with the elements of s, followed by x repeated until the length is reached. 
-function fill<T>(s: seq<T>, x: T, len: nat): (r: seq<T>) 
+// Returns a new sequence with the elements of 's', followed by 'x' repeated until the length is reached. 
+ghost function fill<T>(s: seq<T>, x: T, len: nat): seq<T> 
   requires len >= |s|
-  decreases len - |s|
-  ensures |r| == len
-  ensures r[..|s|] == s
-  ensures forall i :: |s| <= i < len ==> r[i] == x
 {
-    if |s| == len then s else fill(s + [x], x, len)
+    s + seq(len -|s|, i => x)
 }
 
 // Retrieves the same sequence with the last element removed 
-function butlast<T>(s: seq<T>): seq<T>
+ghost function butlast<T>(s: seq<T>): seq<T>
     requires |s| > 0
-    ensures s == butlast(s) + [last(s)]
 { s[..|s|-1] }
 
 // Retrieves the last element of a non-empty sequence
-function last<T>(s: seq<T>): T
+ghost function last<T>(s: seq<T>): T
     requires |s| > 0
 { s[|s|-1] }
 
-// End of sequence utilities
 
 // Test cases checked statically by Dafny (with helper assertions)
 method MoveZeroesToEndTest(){
     var a1 := new int[] [1, 0, 2, 0, 3];
     assert a1[..] == [1, 0, 2, 0, 3]; // proof helper
     assert butlast([1, 0, 2, 0, 3]) == [1, 0, 2, 0]; // proof helper
-    assert butlast([1, 0, 2, 0]) == [1, 0, 2]; // proof helper
     MoveZeroesToEnd(a1);
     assert a1[..] == [1, 2, 3, 0, 0];
  
