dataset/task_id_803.dfy
@@ -1,13 +1,15 @@
 // Checks if a natural number is a perfect square.
-predicate IsPerfectSquare(n: nat) {
+ghost predicate isPerfectSquare(n: nat) {
      exists i : nat ::  i * i == n
 }
-by method
+
+method  IsPerfectSquare(n: nat) returns(result: bool)
+  ensures result == isPerfectSquare(n)
 {
     var i := 0;
     while i * i < n
         invariant 0 <= i <= n
-        invariant forall k :: 0 <= k < i ==> k * k < n
+        invariant i > 0 ==> (i - 1) * (i - 1) < n
     {
         i := i + 1;
     }
@@ -23,16 +25,16 @@ by method
 // Test cases checked statically
 method IsPerfectSquareTest(){
     assert 0 * 0 == 0; // helper
-    assert IsPerfectSquare(0);
+    var r := IsPerfectSquare(0); assert r;
 
     assert 1 * 1 == 1; // helper
-    assert IsPerfectSquare(1);
+    r := IsPerfectSquare(1); assert r;
+    
+    r := IsPerfectSquare(2); assert !r;
+    r := IsPerfectSquare(3); assert !r;
 
-    assert ! IsPerfectSquare(2);
-    assert ! IsPerfectSquare(3);
+    assert 2 * 2 == 4; // helper (witness)
+    r := IsPerfectSquare(4); assert r;
 
-    assert 2 * 2 == 4; // helper
-    assert IsPerfectSquare(4);
-
-    assert ! IsPerfectSquare(1000001);
+    r := IsPerfectSquare(1000001); assert !r;
 }
