dataset/FastExponentiation.dfy
@@ -1,30 +1,40 @@
-// Recursive definiton of x^n.
-function Power(x: real, n: nat) : (p: real) {
-    if n == 0 then 1.0 else x * Power(x, n-1)
-}
-
 // Computes x^n in time O(log n) and space O(1) 
 // using the fast exponentiation algorithm.
 method FastExponentiation(x: real, n: nat) returns (p: real)
   ensures p == Power(x, n)
 {
   p := 1.0; // partial result
-  var mx: real := x; // remaining x
-  var mn: nat := n; // remaining n
+  var mx: real := x; // remaining base (x)
+  var mn: nat := n; // remaining exponent (n)
   while mn > 0 
     invariant Power(x, n) == p * Power(mx, mn)
   {
      PowerLemma(mx, mn/2); // invokes the lemma
-     if mn % 2 == 1 { p := p * mx; } 
+     if mn % 2 == 1 { 
+       p := p * mx; 
+     } 
      mx := mx * mx;
      mn := mn / 2;
     }
 }
 
-// States the property x^(2*n) = (x^2)^(n).
+// Recursive definiton of x^n.
+function Power(x: real, n: nat) : (p: real) {
+    if n == 0 then 1.0 else x * Power(x, n-1)
+}
+
+// Proves (by automtic induction) the property x^(2*n) = (x^2)^(n).
 lemma {:induction n} PowerLemma(x: real, n: nat) 
   ensures Power(x, 2 * n) == Power(x * x, n) 
-{ /*proved automatically by Dafny (automatic induction)!*/ }
+{ 
+  if n == 1 {
+    assert Power(x, 2 * 1) == x * Power(x, 1);
+  }
+  else if n > 1 { 
+    PowerLemma(x, n - 1); 
+  }
+}
+
 
 // Test cases checked statically by Dafny!
 method testPowerDC() {
@@ -32,5 +42,3 @@ method testPowerDC() {
   var p2 := FastExponentiation(2.0, 0); assert p2 == 1.0;
   var p3 := FastExponentiation(-2.0, 1); assert p3 == -2.0;
 }
-
-
