dataset/task_id_732.dfy
@@ -17,8 +17,8 @@ function ReplaceCharWithColon(c: char) : char {
 
 // Auxiliary function that applies a function to every element of a sequence
 // using sequence comprehension.
-ghost function {:opaque} MapSeq<T, E>(s: seq<T>, f: T -> E) : (res: seq<E>) 
-  ensures |res| == |s| && (forall i :: 0 <= i < |s| ==> res[i] == f(s[i]))
+ghost function  MapSeq<T, E>(s: seq<T>, f: T -> E) : (res: seq<E>) 
+  ensures |res| == |s| && (forall i :: 0 <= i < |s| ==> res[i] == f(s[i])) // helper
 {
     seq(|s|, i requires 0 <= i < |s| => f(s[i])) 
 }
